theories/zoo_std/ivar_3.v
@@ -22,8 +22,7 @@ From zoo Require Import
   options.
 
 Implicit Types b : bool.
-Implicit Types l : location.
-Implicit Types v t waiter : val.
+Implicit Types v waiter : val.
 Implicit Types waiters : list val.
 
 Class Ivar3G Σ `{zoo_G : !ZooG Σ} := {
@@ -42,165 +41,736 @@ Proof.
   solve_inG.
 Qed.
 
-Inductive state :=
-  | Unset waiters
-  | Set_ v.
-Implicit Types state : state.
+Module base.
+  Inductive state :=
+    | Unset waiters
+    | Set_ v.
+  Implicit Types state : state.
 
-#[local] Instance state_inhabited : Inhabited state :=
-  populate (Unset []).
+  #[local] Instance state_inhabited : Inhabited state :=
+    populate (Unset []).
 
-#[local] Definition state_to_bool state :=
-  match state with
-  | Unset _ =>
-      false
-  | Set_ _ =>
-      true
-  end.
-#[local] Definition state_to_option state :=
-  match state with
-  | Unset _ =>
-      None
-  | Set_ v =>
-      Some v
-  end.
-#[local] Coercion state_to_val state :=
-  match state with
-  | Unset waiters =>
-      ‘Unset[ lst_to_val waiters ]
-  | Set_ v =>
-      ‘Set( v )
-  end%V.
+  #[local] Definition state_to_bool state :=
+    match state with
+    | Unset _ =>
+        false
+    | Set_ _ =>
+        true
+    end.
+  #[local] Definition state_to_option state :=
+    match state with
+    | Unset _ =>
+        None
+    | Set_ v =>
+        Some v
+    end.
+  #[local] Coercion state_to_val state :=
+    match state with
+    | Unset waiters =>
+        ‘Unset[ lst_to_val waiters ]
+    | Set_ v =>
+        ‘Set( v )
+    end%V.
+
+  Section ivar_3_G.
+    Context `{ivar_3_G : Ivar3G Σ}.
+
+    Implicit Types t : location.
+    Implicit Types Ψ Χ Ξ : val → iProp Σ.
+    Implicit Types Ω : val → val → iProp Σ.
+
+    Record ivar_3_name := {
+      ivar_3_name_lstate : gname ;
+      ivar_3_name_consumer : gname ;
+    }.
+    Implicit Types γ : ivar_3_name.
+
+    #[global] Instance ivar_3_name_eq_dec : EqDecision ivar_3_name :=
+      ltac:(solve_decision).
+    #[global] Instance ivar_3_name_countable :
+      Countable ivar_3_name.
+    Proof.
+      solve_countable.
+    Qed.
+
+    #[local] Definition lstate_unset₁' γ_lstate :=
+      oneshot_pending γ_lstate (DfracOwn (1/3)) ().
+    #[local] Definition lstate_unset₁ γ :=
+      lstate_unset₁' γ.(ivar_3_name_lstate).
+    #[local] Definition lstate_unset₂' γ_lstate :=
+      oneshot_pending γ_lstate (DfracOwn (2/3)) ().
+    #[local] Definition lstate_unset₂ γ :=
+      lstate_unset₂' γ.(ivar_3_name_lstate).
+    #[local] Definition lstate_set γ :=
+      oneshot_shot γ.(ivar_3_name_lstate).
+
+    #[local] Definition consumer_auth' :=
+      subpreds_auth.
+    #[local] Definition consumer_auth γ :=
+      consumer_auth' γ.(ivar_3_name_consumer).
+    #[local] Definition consumer_frag' :=
+      subpreds_frag.
+    #[local] Definition consumer_frag γ :=
+      consumer_frag' γ.(ivar_3_name_consumer).
+
+    #[local] Definition inv_state_unset t γ Ω waiters : iProp Σ :=
+      lstate_unset₁ γ ∗
+      [∗ list] waiter ∈ waiters, Ω #t waiter.
+    #[local] Instance : CustomIpatFormat "inv_state_unset" :=
+      " ( {>;}Hlstate_unset₁ &
+          Hwaiters
+        )
+      ".
+    #[local] Definition inv_state_set γ Ξ v : iProp Σ :=
+      lstate_set γ v ∗
+      □ Ξ v.
+    #[local] Instance : CustomIpatFormat "inv_state_set" :=
+      " ( {>;}#Hlstate_set{_{}} &
+          #HΞ{_{}}
+        )
+      ".
+    #[local] Definition inv_state t γ Ξ Ω state :=
+      match state with
+      | Unset waiters =>
+          inv_state_unset t γ Ω waiters
+      | Set_ v =>
+          inv_state_set γ Ξ v
+      end.
+
+    #[local] Definition inv_inner t γ Ψ Ξ Ω : iProp Σ :=
+      ∃ state,
+      t.[contents] ↦ state ∗
+      consumer_auth γ Ψ (state_to_option state) ∗
+      inv_state t γ Ξ Ω state.
+    #[local] Instance : CustomIpatFormat "inv_inner" :=
+      " ( %state &
+          Ht &
+          Hconsumer_auth &
+          Hstate
+        )
+      ".
+    Definition ivar_3_inv t γ Ψ Ξ Ω : iProp Σ :=
+      inv nroot (inv_inner t γ Ψ Ξ Ω).
+    #[local] Instance : CustomIpatFormat "inv" :=
+      " #Hinv
+      ".
+
+    Definition ivar_3_producer :=
+      lstate_unset₂.
+    #[local] Instance : CustomIpatFormat "producer" :=
+      " Hlstate_unset₂{_{}}
+      ".
+
+    Definition ivar_3_consumer :=
+      consumer_frag.
+    #[local] Instance : CustomIpatFormat "consumer" :=
+      " Hconsumer{}_frag
+      ".
+
+    Definition ivar_3_result :=
+      lstate_set.
+    #[local] Instance : CustomIpatFormat "result" :=
+      " #Hlstate_set{_{}}
+      ".
+    Definition ivar_3_resolved γ : iProp Σ :=
+      ∃ v,
+      ivar_3_result γ v.
+
+    #[global] Instance ivar_3_inv_contractive t γ n :
+      Proper (
+        (pointwise_relation _ (dist_later n)) ==>
+        (pointwise_relation _ (dist_later n)) ==>
+        (pointwise_relation _ (pointwise_relation _ (dist_later n))) ==>
+        (≡{n}≡)
+      ) (ivar_3_inv t γ).
+    Proof.
+      rewrite /ivar_3_inv /inv_inner /inv_state /inv_state_unset /inv_state_set.
+      intros Ψ1 Ψ2 HΨ Ξ1 Ξ2 HΞ Ω1 Ω2 HΩ.
+      repeat (apply HΩ || f_contractive || f_equiv). done.
+    Qed.
+    #[global] Instance ivar_3_inv_proper t γ :
+      Proper (
+        (pointwise_relation _ (≡)) ==>
+        (pointwise_relation _ (≡)) ==>
+        (pointwise_relation _ (pointwise_relation _ (≡))) ==>
+        (≡)
+      ) (ivar_3_inv t γ).
+    Proof.
+      rewrite /ivar_3_inv /inv_inner /inv_state /inv_state_unset /inv_state_set.
+      solve_proper.
+    Qed.
+    #[global] Instance ivar_3_consumer_contractive γ n :
+      Proper (
+        (pointwise_relation _ (dist_later n)) ==>
+        (≡{n}≡)
+      ) (ivar_3_consumer γ).
+    Proof.
+      solve_contractive.
+    Qed.
+    #[global] Instance ivar_3_consumer_proper γ :
+      Proper (
+        (pointwise_relation _ (≡)) ==>
+        (≡)
+      ) (ivar_3_consumer γ).
+    Proof.
+      solve_proper.
+    Qed.
+
+    #[global] Instance ivar_3_producer_timeless γ :
+      Timeless (ivar_3_producer γ).
+    Proof.
+      apply _.
+    Qed.
+    #[global] Instance ivar_3_result_timeless γ v :
+      Timeless (ivar_3_result γ v).
+    Proof.
+      apply _.
+    Qed.
+
+    #[global] Instance ivar_3_inv_persistent t γ Ψ Ξ Ω :
+      Persistent (ivar_3_inv t γ Ψ Ξ Ω).
+    Proof.
+      apply _.
+    Qed.
+    #[global] Instance ivar_3_result_persistent γ v :
+      Persistent (ivar_3_result γ v).
+    Proof.
+      apply _.
+    Qed.
+
+    #[local] Lemma lstate_alloc :
+      ⊢ |==>
+        ∃ γ_lstate,
+        lstate_unset₁' γ_lstate ∗
+        lstate_unset₂' γ_lstate.
+    Proof.
+      iMod oneshot_alloc as "(%γ_lstate & Hpending)".
+      assert (1 = 1/3 + 2/3)%Qp as -> by compute_done.
+      iDestruct "Hpending" as "(Hpending₁ & Hpending₂)".
+      iSteps.
+    Qed.
+    #[local] Lemma lstate_unset₂_exclusive γ :
+      lstate_unset₂ γ -∗
+      lstate_unset₂ γ -∗
+      False.
+    Proof.
+      iIntros "Hpending1 Hpending2".
+      iDestruct (oneshot_pending_valid_2 with "Hpending1 Hpending2") as %(? & _). done.
+    Qed.
+    #[local] Lemma lstate_set_agree γ v1 v2 :
+      lstate_set γ v1 -∗
+      lstate_set γ v2 -∗
+      ⌜v1 = v2⌝.
+    Proof.
+      apply oneshot_shot_agree.
+    Qed.
+    #[local] Lemma lstate_unset₁_set γ v :
+      lstate_unset₁ γ -∗
+      lstate_set γ v -∗
+      False.
+    Proof.
+      apply oneshot_pending_shot.
+    Qed.
+    #[local] Lemma lstate_unset₂_set γ v :
+      lstate_unset₂ γ -∗
+      lstate_set γ v -∗
+      False.
+    Proof.
+      apply oneshot_pending_shot.
+    Qed.
+    #[local] Lemma lstate_update {γ} v :
+      lstate_unset₁ γ -∗
+      lstate_unset₂ γ ==∗
+      lstate_set γ v.
+    Proof.
+      iIntros "Hpending₁ Hpending₂".
+      iCombine "Hpending₁ Hpending₂" as "Hpending".
+      assert (1/3 + 2/3 = 1)%Qp as -> by compute_done.
+      iApply (oneshot_update_shot with "Hpending").
+    Qed.
+
+    #[local] Lemma consumer_alloc Ψ :
+      ⊢ |==>
+        ∃ γ_consumer,
+        consumer_auth' γ_consumer Ψ None ∗
+        consumer_frag' γ_consumer Ψ.
+    Proof.
+      apply subpreds_alloc.
+    Qed.
+    #[local] Lemma consumer_divide {γ Ψ} {state : option val} {Χ} Χs E :
+      ▷ consumer_auth γ Ψ state -∗
+      consumer_frag γ Χ -∗
+      (∀ v, Χ v -∗ [∗ list] Χ ∈ Χs, Χ v) ={E}=∗
+        ▷ consumer_auth γ Ψ state ∗
+        [∗ list] Χ ∈ Χs, consumer_frag γ Χ.
+    Proof.
+      apply subpreds_divide.
+    Qed.
+    #[local] Lemma consumer_produce {γ Ψ} v :
+      consumer_auth γ Ψ None -∗
+      Ψ v -∗
+      consumer_auth γ Ψ (Some v).
+    Proof.
+      apply subpreds_produce.
+    Qed.
+    #[local] Lemma consumer_consume γ Ψ v Χ E :
+      ▷ consumer_auth γ Ψ (Some v) -∗
+      consumer_frag γ Χ ={E}=∗
+        ▷ consumer_auth γ Ψ (Some v) ∗
+        ▷^2 Χ v.
+    Proof.
+      apply subpreds_consume.
+    Qed.
+
+    Lemma ivar_3_producer_exclusive γ :
+      ivar_3_producer γ -∗
+      ivar_3_producer γ -∗
+      False.
+    Proof.
+      iIntros "(:producer =1) (:producer =2)".
+      iApply (lstate_unset₂_exclusive with "Hlstate_unset₂_1 Hlstate_unset₂_2").
+    Qed.
+
+    Lemma ivar_3_consumer_divide {t γ Ψ Ξ Ω Χ} Χs :
+      ivar_3_inv t γ Ψ Ξ Ω -∗
+      ivar_3_consumer γ Χ -∗
+      (∀ v, Χ v -∗ [∗ list] Χ ∈ Χs, Χ v) ={⊤}=∗
+      [∗ list] Χ ∈ Χs, ivar_3_consumer γ Χ.
+    Proof.
+      iIntros "(:inv) (:consumer) H".
+      iInv "Hinv" as "(:inv_inner)".
+      iMod (consumer_divide with "Hconsumer_auth Hconsumer_frag H") as "(Hconsumer_auth & H)".
+      iSplitR "H". { iFrameSteps. }
+      iApply (big_sepL_impl with "H").
+      iSteps.
+    Qed.
+
+    Lemma ivar_3_result_agree γ v1 v2 :
+      ivar_3_result γ v1 -∗
+      ivar_3_result γ v2 -∗
+      ⌜v1 = v2⌝.
+    Proof.
+      iIntros "(:result =1) (:result =2)".
+      iApply (lstate_set_agree with "Hlstate_set_1 Hlstate_set_2").
+    Qed.
+
+    Lemma ivar_3_producer_result γ v :
+      ivar_3_producer γ -∗
+      ivar_3_result γ v -∗
+      False.
+    Proof.
+      iIntros "(:producer =1) (:result =2)".
+      iApply (lstate_unset₂_set with "Hlstate_unset₂_1 Hlstate_set_2").
+    Qed.
+
+    Lemma ivar_3_inv_result t γ Ψ Ξ Ω v :
+      ivar_3_inv t γ Ψ Ξ Ω -∗
+      ivar_3_result γ v ={⊤}=∗
+      ▷ □ Ξ v.
+    Proof.
+      iIntros "(:inv) (:result)".
+      iInv "Hinv" as "(:inv_inner)".
+      destruct state as [waiters | v_].
+      { iDestruct "Hstate" as "(:inv_state_unset >)".
+        iDestruct (lstate_unset₁_set with "Hlstate_unset₁ Hlstate_set") as %[].
+      }
+      iDestruct "Hstate" as "(:inv_state_set =1 >)".
+      iDestruct (lstate_set_agree with "Hlstate_set Hlstate_set_1") as %<-.
+      iSplitL. { iFrameSteps. }
+      iSteps.
+    Qed.
+    Lemma ivar_3_inv_result_consumer t γ Ψ Ξ Ω v Χ :
+      ivar_3_inv t γ Ψ Ξ Ω -∗
+      ivar_3_result γ v -∗
+      ivar_3_consumer γ Χ ={⊤}=∗
+        ▷^2 Χ v ∗
+        ▷ □ Ξ v.
+    Proof.
+      iIntros "(:inv) (:result) (:consumer)".
+      iInv "Hinv" as "(:inv_inner)".
+      destruct state as [v_ |].
+      { iDestruct "Hstate" as "(:inv_state_unset >)".
+        iDestruct (lstate_unset₁_set with "Hlstate_unset₁ Hlstate_set") as %[].
+      }
+      iDestruct "Hstate" as "(:inv_state_set =1 >)".
+      iDestruct (lstate_set_agree with "Hlstate_set Hlstate_set_1") as %<-.
+      iMod (consumer_consume with "Hconsumer_auth Hconsumer_frag") as "(Hconsumer_auth & HΧ)".
+      iSplitR "HΧ". { iFrameSteps. }
+      iSteps.
+    Qed.
+
+    Lemma ivar_3_create_spec Ψ Ξ Ω :
+      {{{
+        True
+      }}}
+        ivar_3_create ()
+      {{{ t γ,
+        RET #t;
+        meta_token t ⊤ ∗
+        ivar_3_inv t γ Ψ Ξ Ω ∗
+        ivar_3_producer γ ∗
+        ivar_3_consumer γ Ψ
+      }}}.
+    Proof.
+      iIntros "%Φ _ HΦ".
+
+      wp_rec.
+      wp_ref t as "Hmeta" "Ht".
+
+      iMod lstate_alloc as "(%γ_lstate & Hlstate_unset₁ & Hlstate_unset₂)".
+      iMod consumer_alloc as "(%γ_consumer & Hconsumer_auth & Hconsumer_frag)".
+
+      pose γ := {|
+        ivar_3_name_lstate := γ_lstate ;
+        ivar_3_name_consumer := γ_consumer ;
+      |}.
+
+      iApply ("HΦ" $! t γ).
+      iFrameSteps. iExists (Unset []). iSteps.
+    Qed.
+
+    Lemma ivar_3_make_spec Ψ Ξ Ω v :
+      {{{
+        ▷ Ψ v ∗
+        ▷ □ Ξ v
+      }}}
+        ivar_3_make v
+      {{{ t γ,
+        RET #t;
+        meta_token t ⊤ ∗
+        ivar_3_inv t γ Ψ Ξ Ω ∗
+        ivar_3_result γ v ∗
+        ivar_3_consumer γ Ψ
+      }}}.
+    Proof.
+      iIntros "%Φ (HΨ & #HΞ) HΦ".
+
+      wp_rec.
+      wp_ref t as "Hmeta" "Ht".
+
+      iMod lstate_alloc as "(%γ_lstate & Hlstate_unset₁ & Hlstate_unset₂)".
+      iMod consumer_alloc as "(%γ_consumer & Hconsumer_auth & Hconsumer_frag)".
+
+      pose γ := {|
+        ivar_3_name_lstate := γ_lstate ;
+        ivar_3_name_consumer := γ_consumer ;
+      |}.
+
+      iMod (lstate_update (γ := γ) v with "Hlstate_unset₁ Hlstate_unset₂") as "#Hlstate_set".
+      iDestruct (consumer_produce (γ := γ) v with "Hconsumer_auth HΨ") as "Hconsumer_auth".
+
+      iApply ("HΦ" $! t γ).
+      iFrameSteps. iExists (Set_ v). iSteps.
+    Qed.
+
+    Lemma ivar_3_is_set_spec t γ Ψ Ξ Ω :
+      {{{
+        ivar_3_inv t γ Ψ Ξ Ω
+      }}}
+        ivar_3_is_set #t
+      {{{ b,
+        RET #b;
+        if b then
+          £ 2 ∗
+          ivar_3_resolved γ
+        else
+          True
+      }}}.
+    Proof.
+      iIntros "%Φ (:inv) HΦ".
+
+      wp_rec credits:"H£".
+      iDestruct (lc_weaken 2 with "H£") as "H£"; first done.
+
+      wp_bind (!_)%E.
+      iInv "Hinv" as "(:inv_inner)".
+      wp_load.
+      iSpecialize ("HΦ" $! (state_to_bool state)).
+      destruct state as [waiters | v].
+
+      - iSplitR "HΦ". { iFrameSteps. }
+        iSteps.
+
+      - iDestruct "Hstate" as "(:inv_state_set)".
+        iSplitR "H£ HΦ". { iFrameSteps. }
+        iStep 5. iExists v. iSteps.
+    Qed.
+    Lemma ivar_3_is_set_spec_result t γ Ψ Ξ Ω v :
+      {{{
+        ivar_3_inv t γ Ψ Ξ Ω ∗
+        ivar_3_result γ v
+      }}}
+        ivar_3_is_set #t
+      {{{
+        RET #true;
+        £ 2
+      }}}.
+    Proof.
+      iIntros "%Φ ((:inv) & (:result)) HΦ".
+
+      wp_rec credits:"H£".
+      iDestruct (lc_weaken 2 with "H£") as "H£"; first done.
+
+      wp_bind (!_)%E.
+      iInv "Hinv" as "(:inv_inner)".
+      wp_load.
+      destruct state as [waiters | v_].
+      { iDestruct "Hstate" as "(:inv_state_unset)".
+        iDestruct (lstate_unset₁_set with "Hlstate_unset₁ Hlstate_set") as %[].
+      }
+      iDestruct "Hstate" as "(:inv_state_set =1)".
+      iDestruct (lstate_set_agree with "Hlstate_set Hlstate_set_1") as %<-. iClear "Hlstate_set_1".
+      iSplitR "H£ HΦ". { iFrameSteps. }
+      iSteps.
+    Qed.
+
+    Lemma ivar_3_try_get_spec t γ Ψ Ξ Ω :
+      {{{
+        ivar_3_inv t γ Ψ Ξ Ω
+      }}}
+        ivar_3_try_get #t
+      {{{ o,
+        RET o : val;
+        if o is Some v then
+          £ 2 ∗
+          ivar_3_result γ v
+        else
+          True
+      }}}.
+    Proof.
+      iIntros "%Φ (:inv) HΦ".
+
+      wp_rec credits:"H£".
+      iDestruct (lc_weaken 2 with "H£") as "H£"; first done.
+
+      wp_bind (!_)%E.
+      iInv "Hinv" as "(:inv_inner)".
+      wp_load.
+      iSpecialize ("HΦ" $! (state_to_option state)).
+      destruct state as [waiters | v].
+
+      - iSplitR "HΦ". { iFrameSteps. }
+        iSteps.
+
+      - iDestruct "Hstate" as "(:inv_state_set)".
+        iSplitR "H£ HΦ". { iFrameSteps. }
+        iSteps.
+    Qed.
+    Lemma ivar_3_try_get_spec_result t γ Ψ Ξ Ω v :
+      {{{
+        ivar_3_inv t γ Ψ Ξ Ω ∗
+        ivar_3_result γ v
+      }}}
+        ivar_3_try_get #t
+      {{{
+        RET Some v : val;
+        £ 2
+      }}}.
+    Proof.
+      iIntros "%Φ ((:inv) & (:result)) HΦ".
+
+      wp_rec credits:"H£".
+      iDestruct (lc_weaken 2 with "H£") as "H£"; first done.
+
+      wp_bind (!_)%E.
+      iInv "Hinv" as "(:inv_inner)".
+      wp_load.
+      destruct state as [waiters | v_].
+      { iDestruct "Hstate" as "(:inv_state_unset)".
+        iDestruct (lstate_unset₁_set with "Hlstate_unset₁ Hlstate_set") as %[].
+      }
+      iDestruct "Hstate" as "(:inv_state_set =1)".
+      iDestruct (lstate_set_agree with "Hlstate_set Hlstate_set_1") as %<-. iClear "Hlstate_set_1".
+      iSplitR "H£ HΦ". { iFrameSteps. }
+      iSteps.
+    Qed.
+
+    Lemma ivar_3_get_spec t γ Ψ Ξ Ω v :
+      {{{
+        ivar_3_inv t γ Ψ Ξ Ω ∗
+        ivar_3_result γ v
+      }}}
+        ivar_3_get #t
+      {{{
+        RET v;
+        £ 2
+      }}}.
+    Proof.
+      iIntros "%Φ ((:inv) & (:result)) HΦ".
+
+      wp_rec credits:"H£".
+      iDestruct (lc_weaken 2 with "H£") as "H£"; first done.
+
+      wp_bind (!_)%E.
+      iInv "Hinv" as "(:inv_inner)".
+      wp_load.
+      destruct state as [waiters | v_].
+      { iDestruct "Hstate" as "(:inv_state_unset)".
+        iDestruct (lstate_unset₁_set with "Hlstate_unset₁ Hlstate_set") as %[].
+      }
+      iDestruct "Hstate" as "(:inv_state_set =1)".
+      iDestruct (lstate_set_agree with "Hlstate_set Hlstate_set_1") as %<-. iClear "Hlstate_set_1".
+      iSplitR "H£ HΦ". { iFrameSteps. }
+      iSteps.
+    Qed.
+
+    Lemma ivar_3_wait_spec t γ Ψ Ξ Ω waiter :
+      {{{
+        ivar_3_inv t γ Ψ Ξ Ω ∗
+        ▷ Ω #t waiter
+      }}}
+        ivar_3_wait #t waiter
+      {{{ o,
+        RET o : val;
+        if o is Some v then
+          £ 2 ∗
+          ivar_3_result γ v ∗
+          Ω #t waiter
+        else
+          True
+      }}}.
+    Proof.
+      iIntros "%Φ ((:inv) & Hwaiter) HΦ".
+      iLöb as "HLöb".
+
+      wp_rec credits:"H£". wp_pures.
+      iDestruct (lc_weaken 2 with "H£") as "H£"; first done.
+
+      wp_bind (!_)%E.
+      iInv "Hinv" as "(:inv_inner)".
+      wp_load.
+      destruct state as [waiters | v].
+
+      - iSplitR "Hwaiter H£ HΦ". { iFrameSteps. }
+        iModIntro.
+
+        wp_pures.
+
+        wp_bind (CAS _ _ _).
+        iInv "Hinv" as "(:inv_inner)".
+        wp_cas as Hcas.
+
+        + iSplitR "Hwaiter HΦ". { iFrameSteps. }
+          iModIntro.
+
+          wp_smart_apply ("HLöb" with "Hwaiter HΦ").
+
+        + destruct state as [waiters' | v]; zoo_simplify.
+          iDestruct "Hstate" as "(:inv_state_unset)".
+          iDestruct (big_sepL_cons_2' _ waiter with "[Hwaiter H£] Hwaiters") as "Hwaiters"; first iSteps.
+          iSplitR "HΦ". { iExists (Unset (waiter :: waiters)). iFrameSteps. }
+          iSpecialize ("HΦ" $! None).
+          iSteps.
+
+      - iDestruct "Hstate" as "(:inv_state_set)".
+        iSplitR "H£ Hwaiter HΦ". { iFrameSteps. }
+        iSpecialize ("HΦ" $! (Some v)).
+        iSteps.
+    Qed.
+
+    Lemma ivar_3_set_spec t γ Ψ Ξ Ω v :
+      {{{
+        ivar_3_inv t γ Ψ Ξ Ω ∗
+        ivar_3_producer γ ∗
+        ▷ Ψ v ∗
+        ▷ □ Ξ v
+      }}}
+        ivar_3_set #t v
+      {{{ waiters,
+        RET lst_to_val waiters;
+        ivar_3_result γ v ∗
+        [∗ list] waiter ∈ waiters, Ω #t waiter
+      }}}.
+    Proof.
+      iIntros "%Φ ((:inv) & (:producer) & HΨ & #HΞ) HΦ".
+
+      wp_rec. wp_pures.
+
+      wp_bind (Xchg _ _).
+      iInv "Hinv" as "(:inv_inner)".
+      wp_xchg.
+      destruct state; last first.
+      { iDestruct "Hstate" as "(:inv_state_set =1)".
+        iDestruct (lstate_unset₂_set with "Hlstate_unset₂ Hlstate_set_1") as %[].
+      }
+      iDestruct "Hstate" as "(:inv_state_unset)".
+      iMod (lstate_update with "Hlstate_unset₁ Hlstate_unset₂") as "#Hlstate_set".
+      iDestruct (consumer_produce with "Hconsumer_auth HΨ") as "Hconsumer_auth".
+      iSplitR "Hwaiters HΦ". { iExists (Set_ v). iSteps. }
+      iSteps.
+    Qed.
+  End ivar_3_G.
+
+  #[global] Opaque ivar_3_inv.
+  #[global] Opaque ivar_3_producer.
+  #[global] Opaque ivar_3_consumer.
+  #[global] Opaque ivar_3_result.
+End base.
+
+From zoo_std Require
+  ivar_3__opaque.
 
 Section ivar_3_G.
   Context `{ivar_3_G : Ivar3G Σ}.
 
+  Implicit Types 𝑡 : location.
+  Implicit Types t : val.
   Implicit Types Ψ Χ Ξ : val → iProp Σ.
   Implicit Types Ω : val → val → iProp Σ.
 
-  Record metadata := {
-    metadata_lstate : gname ;
-    metadata_consumer : gname ;
-  }.
-  Implicit Types γ : metadata.
-
-  #[local] Instance metadata_eq_dec : EqDecision metadata :=
-    ltac:(solve_decision).
-  #[local] Instance metadata_countable :
-    Countable metadata.
-  Proof.
-    solve_countable.
-  Qed.
-
-  #[local] Definition lstate_unset₁' γ_lstate :=
-    oneshot_pending γ_lstate (DfracOwn (1/3)) ().
-  #[local] Definition lstate_unset₁ γ :=
-    lstate_unset₁' γ.(metadata_lstate).
-  #[local] Definition lstate_unset₂' γ_lstate :=
-    oneshot_pending γ_lstate (DfracOwn (2/3)) ().
-  #[local] Definition lstate_unset₂ γ :=
-    lstate_unset₂' γ.(metadata_lstate).
-  #[local] Definition lstate_set γ :=
-    oneshot_shot γ.(metadata_lstate).
-
-  #[local] Definition consumer_auth' :=
-    subpreds_auth.
-  #[local] Definition consumer_auth γ :=
-    consumer_auth' γ.(metadata_consumer).
-  #[local] Definition consumer_frag' :=
-    subpreds_frag.
-  #[local] Definition consumer_frag γ :=
-    consumer_frag' γ.(metadata_consumer).
-
-  #[local] Definition inv_state_unset l γ Ω waiters : iProp Σ :=
-    lstate_unset₁ γ ∗
-    [∗ list] waiter ∈ waiters, Ω #l waiter.
-  #[local] Instance : CustomIpatFormat "inv_state_unset" :=
-    " ( {>;}Hlstate_unset₁ &
-        Hwaiters
-      )
-    ".
-  #[local] Definition inv_state_set γ Ξ v : iProp Σ :=
-    lstate_set γ v ∗
-    □ Ξ v.
-  #[local] Instance : CustomIpatFormat "inv_state_set" :=
-    " ( {>;}#Hlstate_set{_{}} &
-        #HΞ{_{}}
-      )
-    ".
-  #[local] Definition inv_state l γ Ξ Ω state :=
-    match state with
-    | Unset waiters =>
-        inv_state_unset l γ Ω waiters
-    | Set_ v =>
-        inv_state_set γ Ξ v
-    end.
-
-  #[local] Definition inv_inner l γ Ψ Ξ Ω : iProp Σ :=
-    ∃ state,
-    l.[contents] ↦ state ∗
-    consumer_auth γ Ψ (state_to_option state) ∗
-    inv_state l γ Ξ Ω state.
-  #[local] Instance : CustomIpatFormat "inv_inner" :=
-    " ( %state &
-        Hl &
-        Hconsumer_auth &
-        Hstate
-      )
-    ".
   Definition ivar_3_inv t Ψ Ξ Ω : iProp Σ :=
-    ∃ l γ,
-    ⌜t = #l⌝ ∗
-    meta l nroot γ ∗
-    inv nroot (inv_inner l γ Ψ Ξ Ω).
+    ∃ 𝑡 γ,
+    ⌜t = #𝑡⌝ ∗
+    meta 𝑡 nroot γ ∗
+    base.ivar_3_inv 𝑡 γ Ψ Ξ Ω.
   #[local] Instance : CustomIpatFormat "inv" :=
-    " ( %l &
-        %γ &
-        -> &
-        #Hmeta &
-        #Hinv
+    " ( %𝑡{} &
+        %γ{} &
+        {%Heq{};->} &
+        #Hmeta{_{}} &
+        Hinv{_{}}
       )
     ".
 
   Definition ivar_3_producer t : iProp Σ :=
-    ∃ l γ,
-    ⌜t = #l⌝ ∗
-    meta l nroot γ ∗
-    lstate_unset₂ γ.
+    ∃ 𝑡 γ,
+    ⌜t = #𝑡⌝ ∗
+    meta 𝑡 nroot γ ∗
+    base.ivar_3_producer γ.
   #[local] Instance : CustomIpatFormat "producer" :=
-    " ( %l{;_} &
-        %γ{;_} &
-        %Heq{} &
-        #Hmeta{;_} &
-        Hlstate_unset₂{_{}}
+    " ( %𝑡{} &
+        %γ{} &
+        {%Heq{};->} &
+        #Hmeta{_{}} &
+        Hproducer{_{}}
       )
     ".
 
   Definition ivar_3_consumer t Χ : iProp Σ :=
-    ∃ l γ,
-    ⌜t = #l⌝ ∗
-    meta l nroot γ ∗
-    consumer_frag γ Χ.
+    ∃ 𝑡 γ,
+    ⌜t = #𝑡⌝ ∗
+    meta 𝑡 nroot γ ∗
+    base.ivar_3_consumer γ Χ.
   #[local] Instance : CustomIpatFormat "consumer" :=
-    " ( %l{;_} &
-        %γ{;_} &
-        %Heq{} &
-        #Hmeta{;_} &
-        Hconsumer{}_frag
+    " ( %𝑡{} &
+        %γ{} &
+        {%Heq{};->} &
+        #Hmeta{_{}} &
+        Hconsumer{_{}}
       )
     ".
 
   Definition ivar_3_result t v : iProp Σ :=
-    ∃ l γ,
-    ⌜t = #l⌝ ∗
-    meta l nroot γ ∗
-    lstate_set γ v.
+    ∃ 𝑡 γ,
+    ⌜t = #𝑡⌝ ∗
+    meta 𝑡 nroot γ ∗
+    base.ivar_3_result γ v.
   #[local] Instance : CustomIpatFormat "result" :=
-    " ( %l{;_} &
-        %γ{;_} &
-        %Heq{} &
-        #Hmeta{;_} &
-        #Hlstate_set{_{}}
+    " ( %𝑡{} &
+        %γ{} &
+        {%Heq{};->} &
+        #Hmeta{_{}} &
+        Hresult{_{}}
       )
     ".
   Definition ivar_3_resolved t : iProp Σ :=
@@ -215,9 +785,7 @@ Section ivar_3_G.
       (≡{n}≡)
     ) (ivar_3_inv t).
   Proof.
-    rewrite /ivar_3_inv /inv_inner /inv_state /inv_state_unset /inv_state_set.
-    intros Ψ1 Ψ2 HΨ Ξ1 Ξ2 HΞ Ω1 Ω2 HΩ.
-    repeat (apply HΩ || f_contractive || f_equiv). done.
+    solve_proper.
   Qed.
   #[global] Instance ivar_3_inv_proper t :
     Proper (
@@ -227,7 +795,6 @@ Section ivar_3_G.
       (≡)
     ) (ivar_3_inv t).
   Proof.
-    rewrite /ivar_3_inv /inv_inner /inv_state /inv_state_unset /inv_state_set.
     solve_proper.
   Qed.
   #[global] Instance ivar_3_consumer_contractive t n :
@@ -236,7 +803,7 @@ Section ivar_3_G.
       (≡{n}≡)
     ) (ivar_3_consumer t).
   Proof.
-    solve_contractive.
+    solve_proper.
   Qed.
   #[global] Instance ivar_3_consumer_proper t :
     Proper (
@@ -269,98 +836,14 @@ Section ivar_3_G.
     apply _.
   Qed.
 
-  #[local] Lemma lstate_alloc :
-    ⊢ |==>
-      ∃ γ_lstate,
-      lstate_unset₁' γ_lstate ∗
-      lstate_unset₂' γ_lstate.
-  Proof.
-    iMod oneshot_alloc as "(%γ_lstate & Hpending)".
-    assert (1 = 1/3 + 2/3)%Qp as -> by compute_done.
-    iDestruct "Hpending" as "(Hpending₁ & Hpending₂)".
-    iSteps.
-  Qed.
-  #[local] Lemma lstate_unset₂_exclusive γ :
-    lstate_unset₂ γ -∗
-    lstate_unset₂ γ -∗
-    False.
-  Proof.
-    iIntros "Hpending1 Hpending2".
-    iDestruct (oneshot_pending_valid_2 with "Hpending1 Hpending2") as %(? & _). done.
-  Qed.
-  #[local] Lemma lstate_set_agree γ v1 v2 :
-    lstate_set γ v1 -∗
-    lstate_set γ v2 -∗
-    ⌜v1 = v2⌝.
-  Proof.
-    apply oneshot_shot_agree.
-  Qed.
-  #[local] Lemma lstate_unset₁_set γ v :
-    lstate_unset₁ γ -∗
-    lstate_set γ v -∗
-    False.
-  Proof.
-    apply oneshot_pending_shot.
-  Qed.
-  #[local] Lemma lstate_unset₂_set γ v :
-    lstate_unset₂ γ -∗
-    lstate_set γ v -∗
-    False.
-  Proof.
-    apply oneshot_pending_shot.
-  Qed.
-  #[local] Lemma lstate_update {γ} v :
-    lstate_unset₁ γ -∗
-    lstate_unset₂ γ ==∗
-    lstate_set γ v.
-  Proof.
-    iIntros "Hpending₁ Hpending₂".
-    iCombine "Hpending₁ Hpending₂" as "Hpending".
-    assert (1/3 + 2/3 = 1)%Qp as -> by compute_done.
-    iApply (oneshot_update_shot with "Hpending").
-  Qed.
-
-  #[local] Lemma consumer_alloc Ψ :
-    ⊢ |==>
-      ∃ γ_consumer,
-      consumer_auth' γ_consumer Ψ None ∗
-      consumer_frag' γ_consumer Ψ.
-  Proof.
-    apply subpreds_alloc.
-  Qed.
-  #[local] Lemma consumer_divide {γ Ψ} {state : option val} {Χ} Χs E :
-    ▷ consumer_auth γ Ψ state -∗
-    consumer_frag γ Χ -∗
-    (∀ v, Χ v -∗ [∗ list] Χ ∈ Χs, Χ v) ={E}=∗
-      ▷ consumer_auth γ Ψ state ∗
-      [∗ list] Χ ∈ Χs, consumer_frag γ Χ.
-  Proof.
-    apply subpreds_divide.
-  Qed.
-  #[local] Lemma consumer_produce {γ Ψ} v :
-    consumer_auth γ Ψ None -∗
-    Ψ v -∗
-    consumer_auth γ Ψ (Some v).
-  Proof.
-    apply subpreds_produce.
-  Qed.
-  #[local] Lemma consumer_consume γ Ψ v Χ E :
-    ▷ consumer_auth γ Ψ (Some v) -∗
-    consumer_frag γ Χ ={E}=∗
-      ▷ consumer_auth γ Ψ (Some v) ∗
-      ▷^2 Χ v.
-  Proof.
-    apply subpreds_consume.
-  Qed.
-
   Lemma ivar_3_producer_exclusive t :
     ivar_3_producer t -∗
     ivar_3_producer t -∗
     False.
   Proof.
     iIntros "(:producer =1) (:producer =2)". simplify.
-    iDestruct (meta_agree with "Hmeta1 Hmeta2") as %<-.
-    iApply (lstate_unset₂_exclusive with "Hlstate_unset₂_1 Hlstate_unset₂_2").
+    iDestruct (meta_agree with "Hmeta_1 Hmeta_2") as %->.
+    iApply (base.ivar_3_producer_exclusive with "Hproducer_1 Hproducer_2").
   Qed.
 
   Lemma ivar_3_consumer_divide {t Ψ Ξ Ω Χ} Χs :
@@ -369,11 +852,9 @@ Section ivar_3_G.
     (∀ v, Χ v -∗ [∗ list] Χ ∈ Χs, Χ v) ={⊤}=∗
     [∗ list] Χ ∈ Χs, ivar_3_consumer t Χ.
   Proof.
-    iIntros "(:inv) (:consumer) H". injection Heq as <-.
-    iDestruct (meta_agree with "Hmeta Hmeta_") as %<-.
-    iInv "Hinv" as "(:inv_inner)".
-    iMod (consumer_divide with "Hconsumer_auth Hconsumer_frag H") as "(Hconsumer_auth & H)".
-    iSplitR "H". { iFrameSteps. }
+    iIntros "(:inv =1) (:consumer =2) H". simplify.
+    iDestruct (meta_agree with "Hmeta_1 Hmeta_2") as %->.
+    iDestruct (base.ivar_3_consumer_divide with "Hinv_1 Hconsumer_2 H") as "H".
     iApply (big_sepL_impl with "H").
     iSteps.
   Qed.
@@ -394,8 +875,8 @@ Section ivar_3_G.
     ⌜v1 = v2⌝.
   Proof.
     iIntros "(:result =1) (:result =2)". simplify.
-    iDestruct (meta_agree with "Hmeta1 Hmeta2") as %<-.
-    iApply (lstate_set_agree with "Hlstate_set_1 Hlstate_set_2").
+    iDestruct (meta_agree with "Hmeta_1 Hmeta_2") as %->.
+    iApply (base.ivar_3_result_agree with "Hresult_1 Hresult_2").
   Qed.
 
   Lemma ivar_3_producer_result t v :
@@ -404,8 +885,8 @@ Section ivar_3_G.
     False.
   Proof.
     iIntros "(:producer =1) (:result =2)". simplify.
-    iDestruct (meta_agree with "Hmeta1 Hmeta2") as %<-.
-    iApply (lstate_unset₂_set with "Hlstate_unset₂_1 Hlstate_set_2").
+    iDestruct (meta_agree with "Hmeta_1 Hmeta_2") as %->.
+    iApply (base.ivar_3_producer_result with "Hproducer_1 Hresult_2").
   Qed.
 
   Lemma ivar_3_inv_result t Ψ Ξ Ω v :
@@ -413,17 +894,9 @@ Section ivar_3_G.
     ivar_3_result t v ={⊤}=∗
     ▷ □ Ξ v.
   Proof.
-    iIntros "(:inv) (:result)". injection Heq as <-.
-    iDestruct (meta_agree with "Hmeta Hmeta_") as %<-. iClear "Hmeta_".
-    iInv "Hinv" as "(:inv_inner)".
-    destruct state as [waiters | v_].
-    { iDestruct "Hstate" as "(:inv_state_unset >)".
-      iDestruct (lstate_unset₁_set with "Hlstate_unset₁ Hlstate_set") as %[].
-    }
-    iDestruct "Hstate" as "(:inv_state_set =1 >)".
-    iDestruct (lstate_set_agree with "Hlstate_set Hlstate_set_1") as %<-.
-    iSplitL. { iFrameSteps. }
-    iSteps.
+    iIntros "(:inv =1) (:result =2)". simplify.
+    iDestruct (meta_agree with "Hmeta_1 Hmeta_2") as %<-.
+    iApply (base.ivar_3_inv_result with "Hinv_1 Hresult_2").
   Qed.
   Lemma ivar_3_inv_result' t Ψ Ξ Ω v :
     £ 1 -∗
@@ -442,20 +915,10 @@ Section ivar_3_G.
       ▷^2 Χ v ∗
       ▷ □ Ξ v.
   Proof.
-    iIntros "(:inv) (:result)". injection Heq as <-.
-    iDestruct (meta_agree with "Hmeta Hmeta_") as %<-. iClear "Hmeta_".
-    iIntros "(:consumer)". injection Heq as <-.
-    iDestruct (meta_agree with "Hmeta Hmeta_") as %<-. iClear "Hmeta_".
-    iInv "Hinv" as "(:inv_inner)".
-    destruct state as [v_ |].
-    { iDestruct "Hstate" as "(:inv_state_unset >)".
-      iDestruct (lstate_unset₁_set with "Hlstate_unset₁ Hlstate_set") as %[].
-    }
-    iDestruct "Hstate" as "(:inv_state_set =1 >)".
-    iDestruct (lstate_set_agree with "Hlstate_set Hlstate_set_1") as %<-.
-    iMod (consumer_consume with "Hconsumer_auth Hconsumer_frag") as "(Hconsumer_auth & HΧ)".
-    iSplitR "HΧ". { iFrameSteps. }
-    iSteps.
+    iIntros "(:inv =1) (:result =2) (:consumer =3)". simplify.
+    iDestruct (meta_agree with "Hmeta_1 Hmeta_2") as %->.
+    iDestruct (meta_agree with "Hmeta_2 Hmeta_3") as %<-.
+    iApply (base.ivar_3_inv_result_consumer with "Hinv_1 Hresult_2 Hconsumer_3").
   Qed.
   Lemma ivar_3_inv_result_consumer' t Ψ Ξ Ω v Χ :
     £ 2 -∗
@@ -486,21 +949,10 @@ Section ivar_3_G.
   Proof.
     iIntros "%Φ _ HΦ".
 
-    wp_rec.
-    wp_ref l as "Hmeta" "Hl".
-
-    iMod lstate_alloc as "(%γ_lstate & Hlstate_unset₁ & Hlstate_unset₂)".
-    iMod consumer_alloc as "(%γ_consumer & Hconsumer_auth & Hconsumer_frag)".
-
-    pose γ := {|
-      metadata_lstate := γ_lstate ;
-      metadata_consumer := γ_consumer ;
-    |}.
+    iApply wp_fupd.
+    wp_apply (base.ivar_3_create_spec with "[//]") as (𝑡 γ) "(Hmeta & Hinv & Hproducer & Hconsumer)".
     iMod (meta_set γ with "Hmeta") as "#Hmeta"; first done.
-
-    iApply "HΦ".
-    iSplitR "Hconsumer_frag Hlstate_unset₂"; last iSteps.
-    iSteps. iExists (Unset []). iSteps.
+    iSteps.
   Qed.
 
   Lemma ivar_3_make_spec Ψ Ξ Ω v :
@@ -518,24 +970,10 @@ Section ivar_3_G.
   Proof.
     iIntros "%Φ (HΨ & #HΞ) HΦ".
 
-    wp_rec.
-    wp_ref l as "Hmeta" "Hl".
-
-    iMod lstate_alloc as "(%γ_lstate & Hlstate_unset₁ & Hlstate_unset₂)".
-    iMod consumer_alloc as "(%γ_consumer & Hconsumer_auth & Hconsumer_frag)".
-
-    pose γ := {|
-      metadata_lstate := γ_lstate ;
-      metadata_consumer := γ_consumer ;
-    |}.
+    iApply wp_fupd.
+    wp_apply (base.ivar_3_make_spec with "[$]") as (𝑡 γ) "(Hmeta & Hinv & Hproducer & Hconsumer)".
     iMod (meta_set γ with "Hmeta") as "#Hmeta"; first done.
-
-    iMod (lstate_update (γ := γ) v with "Hlstate_unset₁ Hlstate_unset₂") as "#Hlstate_set".
-    iDestruct (consumer_produce (γ := γ) v with "Hconsumer_auth HΨ") as "Hconsumer_auth".
-
-    iApply "HΦ".
-    iSplitR "Hconsumer_frag Hlstate_set"; last iSteps.
-    iSteps. iExists (Set_ v). iSteps.
+    iSteps.
   Qed.
 
   Lemma ivar_3_is_set_spec t Ψ Ξ Ω :
@@ -554,21 +992,8 @@ Section ivar_3_G.
   Proof.
     iIntros "%Φ (:inv) HΦ".
 
-    wp_rec credits:"H£".
-    iDestruct (lc_weaken 2 with "H£") as "H£"; first done.
-
-    wp_bind (!_)%E.
-    iInv "Hinv" as "(:inv_inner)".
-    wp_load.
-    iSpecialize ("HΦ" $! (state_to_bool state)).
-    destruct state as [waiters | v].
-
-    - iSplitR "HΦ". { iFrameSteps. }
-      iSteps.
-
-    - iDestruct "Hstate" as "(:inv_state_set)".
-      iSplitR "H£ HΦ". { iFrameSteps. }
-      iStep 5. iExists v. iSteps.
+    wp_apply (base.ivar_3_is_set_spec with "[$]") as (b) "Hb".
+    rewrite /ivar_3_resolved. destruct b; iSteps.
   Qed.
   Lemma ivar_3_is_set_spec_result t Ψ Ξ Ω v :
     {{{
@@ -581,23 +1006,10 @@ Section ivar_3_G.
       £ 2
     }}}.
   Proof.
-    iIntros "%Φ ((:inv) & (:result)) HΦ". injection Heq as <-.
-    iDestruct (meta_agree with "Hmeta Hmeta_") as %<-. iClear "Hmeta_".
+    iIntros "%Φ ((:inv =1) & (:result =2)) HΦ". simplify.
+    iDestruct (meta_agree with "Hmeta_1 Hmeta_2") as %->. iClear "Hmeta_1".
 
-    wp_rec credits:"H£".
-    iDestruct (lc_weaken 2 with "H£") as "H£"; first done.
-
-    wp_bind (!_)%E.
-    iInv "Hinv" as "(:inv_inner)".
-    wp_load.
-    destruct state as [waiters | v_].
-    { iDestruct "Hstate" as "(:inv_state_unset)".
-      iDestruct (lstate_unset₁_set with "Hlstate_unset₁ Hlstate_set") as %[].
-    }
-    iDestruct "Hstate" as "(:inv_state_set =1)".
-    iDestruct (lstate_set_agree with "Hlstate_set Hlstate_set_1") as %<-. iClear "Hlstate_set_1".
-    iSplitR "H£ HΦ". { iFrameSteps. }
-    iSteps.
+    wp_apply (base.ivar_3_is_set_spec_result with "[$] HΦ").
   Qed.
 
   Lemma ivar_3_try_get_spec t Ψ Ξ Ω :
@@ -616,21 +1028,9 @@ Section ivar_3_G.
   Proof.
     iIntros "%Φ (:inv) HΦ".
 
-    wp_rec credits:"H£".
-    iDestruct (lc_weaken 2 with "H£") as "H£"; first done.
-
-    wp_bind (!_)%E.
-    iInv "Hinv" as "(:inv_inner)".
-    wp_load.
-    iSpecialize ("HΦ" $! (state_to_option state)).
-    destruct state as [waiters | v].
-
-    - iSplitR "HΦ". { iFrameSteps. }
-      iSteps.
-
-    - iDestruct "Hstate" as "(:inv_state_set)".
-      iSplitR "H£ HΦ". { iFrameSteps. }
-      iSteps.
+    wp_apply (base.ivar_3_try_get_spec with "[$]") as (o) "Ho".
+    iSpecialize ("HΦ" $! o).
+    destruct o; iSteps.
   Qed.
   Lemma ivar_3_try_get_spec_result t Ψ Ξ Ω v :
     {{{
@@ -643,23 +1043,10 @@ Section ivar_3_G.
       £ 2
     }}}.
   Proof.
-    iIntros "%Φ ((:inv) & (:result)) HΦ". injection Heq as <-.
-    iDestruct (meta_agree with "Hmeta Hmeta_") as %<-. iClear "Hmeta_".
+    iIntros "%Φ ((:inv =1) & (:result =2)) HΦ". simplify.
+    iDestruct (meta_agree with "Hmeta_1 Hmeta_2") as %->. iClear "Hmeta_1".
 
-    wp_rec credits:"H£".
-    iDestruct (lc_weaken 2 with "H£") as "H£"; first done.
-
-    wp_bind (!_)%E.
-    iInv "Hinv" as "(:inv_inner)".
-    wp_load.
-    destruct state as [waiters | v_].
-    { iDestruct "Hstate" as "(:inv_state_unset)".
-      iDestruct (lstate_unset₁_set with "Hlstate_unset₁ Hlstate_set") as %[].
-    }
-    iDestruct "Hstate" as "(:inv_state_set =1)".
-    iDestruct (lstate_set_agree with "Hlstate_set Hlstate_set_1") as %<-. iClear "Hlstate_set_1".
-    iSplitR "H£ HΦ". { iFrameSteps. }
-    iSteps.
+    wp_apply (base.ivar_3_try_get_spec_result with "[$] HΦ").
   Qed.
 
   Lemma ivar_3_get_spec t Ψ Ξ Ω v :
@@ -673,23 +1060,10 @@ Section ivar_3_G.
       £ 2
     }}}.
   Proof.
-    iIntros "%Φ ((:inv) & (:result)) HΦ". injection Heq as <-.
-    iDestruct (meta_agree with "Hmeta Hmeta_") as %<-. iClear "Hmeta_".
+    iIntros "%Φ ((:inv =1) & (:result =2)) HΦ". simplify.
+    iDestruct (meta_agree with "Hmeta_1 Hmeta_2") as %->. iClear "Hmeta_1".
 
-    wp_rec credits:"H£".
-    iDestruct (lc_weaken 2 with "H£") as "H£"; first done.
-
-    wp_bind (!_)%E.
-    iInv "Hinv" as "(:inv_inner)".
-    wp_load.
-    destruct state as [waiters | v_].
-    { iDestruct "Hstate" as "(:inv_state_unset)".
-      iDestruct (lstate_unset₁_set with "Hlstate_unset₁ Hlstate_set") as %[].
-    }
-    iDestruct "Hstate" as "(:inv_state_set =1)".
-    iDestruct (lstate_set_agree with "Hlstate_set Hlstate_set_1") as %<-. iClear "Hlstate_set_1".
-    iSplitR "H£ HΦ". { iFrameSteps. }
-    iSteps.
+    wp_apply (base.ivar_3_get_spec with "[$] HΦ").
   Qed.
 
   Lemma ivar_3_wait_spec t Ψ Ξ Ω waiter :
@@ -709,41 +1083,10 @@ Section ivar_3_G.
     }}}.
   Proof.
     iIntros "%Φ ((:inv) & Hwaiter) HΦ".
-    iLöb as "HLöb".
 
-    wp_rec credits:"H£". wp_pures.
-    iDestruct (lc_weaken 2 with "H£") as "H£"; first done.
-
-    wp_bind (!_)%E.
-    iInv "Hinv" as "(:inv_inner)".
-    wp_load.
-    destruct state as [waiters | v].
-
-    - iSplitR "Hwaiter H£ HΦ". { iFrameSteps. }
-      iModIntro.
-
-      wp_pures.
-
-      wp_bind (CAS _ _ _).
-      iInv "Hinv" as "(:inv_inner)".
-      wp_cas as Hcas.
-
-      + iSplitR "Hwaiter HΦ". { iFrameSteps. }
-        iModIntro.
-
-        wp_smart_apply ("HLöb" with "Hwaiter HΦ").
-
-      + destruct state as [waiters' | v]; zoo_simplify.
-        iDestruct "Hstate" as "(:inv_state_unset)".
-        iDestruct (big_sepL_cons_2' _ waiter with "[Hwaiter H£] Hwaiters") as "Hwaiters"; first iSteps.
-        iSplitR "HΦ". { iExists (Unset (waiter :: waiters)). iFrameSteps. }
-        iSpecialize ("HΦ" $! None).
-        iSteps.
-
-    - iDestruct "Hstate" as "(:inv_state_set)".
-      iSplitR "H£ Hwaiter HΦ". { iFrameSteps. }
-      iSpecialize ("HΦ" $! (Some v)).
-      iSteps.
+    wp_apply (base.ivar_3_wait_spec with "[$]") as (o) "Ho".
+    iSpecialize ("HΦ" $! o).
+    destruct o; iSteps.
   Qed.
 
   Lemma ivar_3_set_spec t Ψ Ξ Ω v :
@@ -760,28 +1103,13 @@ Section ivar_3_G.
       [∗ list] waiter ∈ waiters, Ω t waiter
     }}}.
   Proof.
-    iIntros "%Φ ((:inv) & (:producer) & HΨ & #HΞ) HΦ". injection Heq as <-.
-    iDestruct (meta_agree with "Hmeta Hmeta_") as %<-. iClear "Hmeta_".
+    iIntros "%Φ ((:inv =1) & (:producer =2) & HΨ & HΞ) HΦ". simplify.
+    iDestruct (meta_agree with "Hmeta_1 Hmeta_2") as %->. iClear "Hmeta_1".
 
-    wp_rec. wp_pures.
-
-    wp_bind (Xchg _ _).
-    iInv "Hinv" as "(:inv_inner)".
-    wp_xchg.
-    destruct state; last first.
-    { iDestruct "Hstate" as "(:inv_state_set =1)".
-      iDestruct (lstate_unset₂_set with "Hlstate_unset₂ Hlstate_set_1") as %[].
-    }
-    iDestruct "Hstate" as "(:inv_state_unset)".
-    iMod (lstate_update with "Hlstate_unset₁ Hlstate_unset₂") as "#Hlstate_set".
-    iDestruct (consumer_produce with "Hconsumer_auth HΨ") as "Hconsumer_auth".
-    iSplitR "Hwaiters HΦ". { iExists (Set_ v). iSteps. }
+    wp_apply (base.ivar_3_set_spec with "[$]").
     iSteps.
   Qed.
 End ivar_3_G.
-
-From zoo_std Require
-  ivar_3__opaque.
 
 #[global] Opaque ivar_3_inv.
 #[global] Opaque ivar_3_producer.
